custom ST effect: done but bad performances

fstar/Effect.fst
@@ -2,46 +2,180 @@ module Effect
 
 
 open FStar.Preorder
+module U8 = FStar.UInt8
+module U16 = FStar.UInt16
+module P = FStar.Preorder
 
 module W = FStar.Monotonic.Witnessed
 open FStar.Monotonic.Pure
 
 // concurrent ST monad definition with a type for configuration
-let cst_pre (config state:Type0) = config -> (state -> Type0) -> Type0
-let cst_post (config state:Type0) (a:Type) = config -> (state -> Type0) -> a -> state -> Type0
+let cst_pre (state:Type0) = (state -> Type0) -> Type0
+let cst_post (state:Type0) (a:Type) = (state -> Type0) -> a -> state -> Type0
 
-type repr (a:Type) (config state:Type0) (pre:cst_pre config state) (post:cst_post config state a) =
-  (c:config) -> (p:(state -> Type0) {pre c p}) -> 
+type repr (a:Type) (state:Type0) (pre:cst_pre state) (post:cst_post state a) =
+  (p:(state -> Type0) {pre p}) -> 
     //Pure (a & (state -> state)) (requires pre c p) (ensures fun out ->
     //  forall s. p s ==> post c p out._1 (out._2 s)
     //)
-    out:(a & (state -> state)){forall s. p s ==> post c p out._1 (out._2 s)}
+    out:(a & (s:state{p s} -> state)){forall s. p s ==> post p out._1 (out._2 s)}
 
 inline_for_extraction
-let return (a:Type) (x:a) (config state:Type0) :
-  repr a config state (fun _ _ -> True) (fun _ p out s -> p s /\ x == out) =
-  fun c p -> (x, (fun (s:state) -> s))
+let return (a:Type) (x:a) (state:Type0) :
+  repr a state (fun _ -> True) (fun p out s -> p s /\ x == out) =
+  fun p -> (x, (fun (s:state{p s}) -> s))
 
-let bind (a b:Type) (config state:Type0)
-  (pre_f:cst_pre config state)
-  (post_f:cst_post config state a)
-  (pre_g:a -> cst_pre config state)
-  (post_g:a -> cst_post config state b)
-  (f:repr a config state pre_f post_f)
-  (g:(x:a) -> repr b config state (pre_g x) (post_g x))
-  : repr b config state
-    (fun c p -> pre_f c p /\ (forall x. pre_g x c (post_f c p x)))
-    (fun c p x s -> exists y. post_g y c (post_f c p y) x s)
-  = fun c p ->
-  let (x, f1) = f c p in
-  let (y, f2) = g x c (post_f c p x) in
+let bind (a b:Type) (state:Type0)
+  (pre_f:cst_pre state)
+  (post_f:cst_post state a)
+  (pre_g:a -> cst_pre state)
+  (post_g:a -> cst_post state b)
+  (f:repr a state pre_f post_f)
+  (g:(x:a) -> repr b state (pre_g x) (post_g x))
+  : repr b state
+    (fun p -> pre_f p /\ (forall x. pre_g x (post_f p x)))
+    (fun p x s -> exists y. post_g y (post_f p y) x s)
+  = fun p ->
+  let (x, f1) = f p in
+  let (y, f2) = g x (post_f p x) in
   (y, (fun s -> f2 (f1 s)))
 
-#push-options "--query_stats"
+let ite_pre (#state:Type) (pre pre':cst_pre state) (b:bool)
+  : cst_pre state = fun p ->
+  (b ==> pre p) /\ ((~b) ==> pre' p)
 
-total reifiable reflectable
+let ite_post (#a:Type) (#state:Type) (post post':cst_post state a) (b:bool)
+  : cst_post state a = fun p out s ->
+  (b ==> post p out s) /\ ((~b) ==> post' p out s)
+
+let if_then_else
+  (a:Type) (state:Type0)
+  (pre:cst_pre state)
+  (post:cst_post state a)
+  (pre':cst_pre state)
+  (post':cst_post state a)
+  (f:repr a state pre  post )
+  (g:repr a state pre' post') (b:bool)
+  = repr a state (ite_pre pre pre' b) (ite_post post post' b)
+
+unfold let stronger
+  (#a:Type) (#state:Type0)
+  (pre pre':cst_pre state)
+  (post post':cst_post state a)
+  : Type0 =
+  (forall p. pre' p ==> pre p) /\
+  (forall p out s. pre p /\ post p out s ==> post' p out s)
+
+let subcomp (a:Type) (state:Type0)
+  (pre pre': cst_pre state)
+  (post post': cst_post state a)
+  (f:repr a state pre post)
+  // : repr u#uu a config state pre post
+  : Pure (repr a state pre' post')
+    (requires stronger pre pre' post post')
+    (ensures fun _ -> True)
+  = f
+
+
+total reifiable
+reflectable
 effect {
-  TEST (a:Type) (config state:Type0) (_:cst_pre config state) (_:cst_post config state a)
-  with {repr; return; bind}
+  ST (a:Type) 
+    ([@@@ effect_param] state:Type0)
+    (_:cst_pre state)
+    (_:cst_post state a)
+  with {repr; return; bind; subcomp; if_then_else}
 }
 
+let lift_pure (a:Type) (state:Type0) (wp:pure_wp a) (f:unit -> PURE a wp) :
+  repr a state (fun _ -> wp (fun _ -> True)) (fun p r s -> p s /\ ~(wp (fun x -> x =!= r)))
+  = elim_pure_wp_monotonicity_forall ();
+  fun _ -> (f (), (fun s -> s))
+
+sub_effect PURE ~> ST = lift_pure
+
+noeq type state_t : Type0 = {
+     bytemap: Map.t U16.t U8.t;
+  }
+
+noeq type config : Type = {
+     r0: P.preorder state_t;
+     r1: P.preorder state_t;
+  }
+
+let state_prop = state_t -> Type0
+
+// pre-condition for write the value `v` at the index `k`
+let write_pre0 (c:config) (k:U16.t) (v:U8.t) (p0:state_prop) : prop =
+  forall s. p0 s ==> c.r0 s {bytemap = Map.upd s.bytemap k v}
+
+let write_post0 (c:config) (k:U16.t) (v:U8.t) (p0:state_prop) (y:state_t) : prop = 
+  exists x. p0 x /\ c.r1 {bytemap = Map.upd x.bytemap k v} y
+
+
+let read_post0 (c:config) (k:U16.t) (p0:state_prop) (v:U8.t) (y:state_t) : prop =
+  exists x. p0 x /\ Map.sel x.bytemap k == v /\ c.r1 x y
+
+let read_post0' (c:config) (k:U16.t) (p0:state_prop) (v:U8.t) : prop =
+  exists s. p0 s /\ Map.sel s.bytemap k == v
+
+
+assume val read0 (#c:config) (k:U16.t) :
+  ST U8.t state_t
+    (fun p0 -> True)
+    (fun p0 v s -> read_post0 c k p0 v s)
+
+assume val write0 (#c:config) (k:U16.t) (v:U8.t) :
+  ST unit state_t
+    (write_pre0 c k v)
+    (fun p0 _ s -> write_post0 c k v p0 s)
+
+
+assume val cas0 (c:config) (key:U16.t) (old_v new_v:U8.t) :
+  ST (option U8.t) state_t
+    (fun p0 -> True)
+    (fun p0 r s ->
+      (None? r ==>
+        write_pre0 c key new_v (fun s -> p0 s /\ Map.sel s.bytemap key == old_v) /\
+        write_post0 c key new_v (fun s -> p0 s /\ Map.sel s.bytemap key == old_v) s
+      ) /\ (Some? r ==> (r <> Some old_v /\
+        read_post0 c key p0 (match r with | Some x -> x) s// /\
+        //read_post0' c key p0 (match r with | Some x -> x)
+      ))
+    )
+
+let c0 = {
+    r0 = (fun s1 s2 -> s1 == s2 \/
+      ((
+        Map.sel s1.bytemap 0us == 0uy \/
+        Map.sel s1.bytemap 0us == 1uy
+      ) /\ (
+        Map.sel s2.bytemap 0us == 0uy \/
+        Map.sel s2.bytemap 0us == 1uy
+      )
+    ));
+    r1 = (fun s1 s2 -> s1 == s2 \/ (
+      (
+        Map.sel s1.bytemap 0us == 0uy \/
+        Map.sel s1.bytemap 0us == 2uy
+      ) /\ (
+        Map.sel s1.bytemap 0us == 0uy \/
+        Map.sel s2.bytemap 0us == 2uy
+      )
+    ))
+  }
+
+let c1 = {
+    r1 = c0.r0;
+    r0 = c0.r1
+  }
+
+#push-options "--z3rlimit 50"
+let prog0 (_:unit) :
+  ST unit state_t (fun _ -> True) (fun _ _ _ -> True) =
+  match cas0 c0 0us 0uy 1uy with
+  | Some v -> ()
+  | None ->
+    write0 #c0 1us 42uy;
+    write0 #c0 2us 43uy;
+    write0 #c0 0us 0uy
